src3.0/SoftBound/sb_ds_trans_axioms.v
@@ -198,9 +198,9 @@ Axiom set_mmetadata_fn__prop : forall TD Mem1 lc2 als2 Mem2 S2 Ps2 F2
   (forall b2, Mem.valid_block Mem1 b2 -> Mem.valid_block Mem2 b2) /\
   (forall b0, Mem.bounds Mem1 b0 = Mem.bounds Mem2 b0).
 
-Axiom dstk_spec : forall TD M, 
-  external_intrinsics.callExternalOrIntrinsics TD M dstk_fid 
-    (deckind_external eid_other) nil = Some (None, M).
+Axiom dstk_spec : forall TD gl M, 
+  callExternalOrIntrinsics TD gl M dstk_fid dstk_typ Nil_list_typ
+    (deckind_external eid_other) nil = Some (None, events.E0, M).
 
 Axiom dstk_is_found : forall TD Ps gl lc fs, 
   exists fv,
@@ -212,20 +212,24 @@ Axiom dstk_is_found : forall TD Ps gl lc fs,
 Definition int2GV n :=
   (Vint 31 (Int.repr 31 (INTEGER.to_Z n)), AST.Mint 31)::nil.
 
-Axiom stk_ret_sim : forall TD M1 M2 mi mgb MM bgv egv,
+Axiom stk_ret_sim : forall TD gl M1 M2 mi mgb MM bgv egv,
   mem_simulation mi TD mgb MM M1 M2 ->
   wf_sb_mi mgb mi M1 M2 ->
   exists M2',  exists M2'',
-    external_intrinsics.callExternalOrIntrinsics TD M2 ssb_fid 
-      (deckind_external eid_other) (bgv::int2GV 0%Z::nil) = Some (None, M2') /\
-    external_intrinsics.callExternalOrIntrinsics TD M2' sse_fid 
-      (deckind_external eid_other) (egv::int2GV 0%Z::nil) = Some (None, M2'') /\
+    callExternalOrIntrinsics TD gl M2 ssb_fid ssb_typ Nil_list_typ
+      (deckind_external eid_other) (bgv::int2GV 0%Z::nil) 
+        = Some (None, events.E0, M2') /\
+    callExternalOrIntrinsics TD gl M2' sse_fid sse_typ Nil_list_typ
+      (deckind_external eid_other) (egv::int2GV 0%Z::nil) 
+        = Some (None, events.E0, M2'') /\
     mem_simulation mi TD mgb MM M1 M2'' /\
     wf_sb_mi mgb mi M1 M2'' /\
-    external_intrinsics.callExternalOrIntrinsics TD M2'' gsb_fid 
-      (deckind_external eid_other) [int2GV 0%Z] = Some (Some bgv, M2'') /\
-    external_intrinsics.callExternalOrIntrinsics TD M2'' gse_fid 
-      (deckind_external eid_other) [int2GV 0%Z] = Some (Some egv, M2'').
+    callExternalOrIntrinsics TD gl M2'' gsb_fid gsb_typ Nil_list_typ
+      (deckind_external eid_other) [int2GV 0%Z] 
+        = Some (Some bgv, events.E0, M2'') /\
+    callExternalOrIntrinsics TD gl M2'' gse_fid gse_typ Nil_list_typ
+      (deckind_external eid_other) [int2GV 0%Z] 
+        = Some (Some egv, events.E0, M2'').
 
 Axiom ssb_is_found : forall TD Ps gl lc fs, 
   exists fv,
@@ -255,19 +259,19 @@ Axiom gse_is_found : forall TD Ps gl lc fs,
     (fdec_intro (fheader_intro sb_fnattrs gse_typ gse_fid nil false)
       (deckind_external eid_other)).
 
-Axiom free_doesnt_change_gsb : forall TD M1 z gv M2 als,
-  external_intrinsics.callExternalOrIntrinsics TD M1 gsb_fid 
-    (deckind_external eid_other) [int2GV z] = ret (ret gv, M1) ->
+Axiom free_doesnt_change_gsb : forall TD M1 z gv M2 als gl,
+  callExternalOrIntrinsics TD gl M1 gsb_fid gsb_typ Nil_list_typ
+    (deckind_external eid_other) [int2GV z] = ret (ret gv, events.E0, M1) ->
   free_allocas TD M1 als = ret M2 ->
-  external_intrinsics.callExternalOrIntrinsics TD M2 gsb_fid 
-    (deckind_external eid_other) [int2GV z] = ret (ret gv, M2).
+  callExternalOrIntrinsics TD gl M2 gsb_fid gsb_typ Nil_list_typ
+    (deckind_external eid_other) [int2GV z] = ret (ret gv, events.E0, M2).
 
-Axiom free_doesnt_change_gse : forall TD M1 z gv M2 als,
-  external_intrinsics.callExternalOrIntrinsics TD M1 gse_fid 
-    (deckind_external eid_other) [int2GV z] = ret (ret gv, M1) ->
+Axiom free_doesnt_change_gse : forall TD M1 z gv M2 als gl,
+  callExternalOrIntrinsics TD gl M1 gse_fid gse_typ Nil_list_typ
+    (deckind_external eid_other) [int2GV z] = ret (ret gv, events.E0, M1) ->
   free_allocas TD M1 als = ret M2 ->
-  external_intrinsics.callExternalOrIntrinsics TD M2 gse_fid 
-    (deckind_external eid_other) [int2GV z] = ret (ret gv, M2).
+  callExternalOrIntrinsics TD gl M2 gse_fid gse_typ Nil_list_typ
+    (deckind_external eid_other) [int2GV z] = ret (ret gv, events.E0, M2).
 
 Axiom wrapper_fid_is_identical : forall fid, wrapper_fid fid = fid.
 
@@ -326,12 +330,12 @@ Axiom lookupExFdecViaPtr_isnt_callLib : forall Ps1 fs1 fv fa rt fid la va dck,
 Axiom shadow_stack_exfdec : forall la lc' mi lc2 lp cs1 nts los fptr
     Mem0 MM mgb fa rt fid va fs2 gl2 als2 tmn2 S2 Ps2 B2 cs2' dck
     fv ft noret0 ca rid cs22 cs23 bs2 fh2 ECs2 M2 Mem' rm rm2
-    bs1 fh1 lc oresult rm' gvs,
+    bs1 fh1 lc oresult rm' gvs tr,
   wf_sb_mi mgb mi Mem0 M2 /\
   mem_simulation mi (los, nts) mgb MM Mem0 M2 /\
   reg_simulation mi (los, nts) gl2 (fdef_intro fh1 bs1) rm rm2 lc lc2 ->
-  external_intrinsics.callExternalOrIntrinsics (los,nts) Mem0 fid 
-    dck gvs = ret (oresult, Mem') ->
+  callExternalOrIntrinsics (los,nts) gl2 Mem0 fid rt (args2Typs la)
+    dck gvs = ret (oresult, tr, Mem') ->
   SBspec.exCallUpdateLocals (los, nts) ft noret0 rid oresult lc rm = 
     ret (lc', rm') ->
   ret cs1 = trans_params rm2 lp 1 ->
@@ -355,19 +359,19 @@ Axiom shadow_stack_exfdec : forall la lc' mi lc2 lp cs1 nts los fptr
   mem_simulation mi (los, nts) mgb MM Mem' M2' /\
   reg_simulation mi (los, nts) gl2 (fdef_intro fh1 bs1) rm' rm2 lc' lc2'.
 
-Axiom free_allocas_preserves_gsb : forall M2 TD als2 M2' lp re,
+Axiom free_allocas_preserves_gsb : forall M2 TD als2 M2' lp re gl,
   free_allocas TD M2 als2 = ret M2' ->
-  external_intrinsics.callExternalOrIntrinsics TD M2 gsb_fid 
-    (deckind_external eid_other) lp = Some (re, M2) ->
-  external_intrinsics.callExternalOrIntrinsics TD M2' gsb_fid 
-    (deckind_external eid_other) lp = Some (re, M2').
+  callExternalOrIntrinsics TD gl M2 gsb_fid gsb_typ Nil_list_typ
+    (deckind_external eid_other) lp = Some (re, events.E0, M2) ->
+  callExternalOrIntrinsics TD gl M2' gsb_fid gsb_typ Nil_list_typ
+    (deckind_external eid_other) lp = Some (re, events.E0, M2').
 
-Axiom free_allocas_preserves_gse : forall M2 TD als2 M2' lp re,
+Axiom free_allocas_preserves_gse : forall M2 TD als2 M2' lp re gl,
   free_allocas TD M2 als2 = ret M2' ->
-  external_intrinsics.callExternalOrIntrinsics TD M2 gse_fid 
-    (deckind_external eid_other) lp = Some (re, M2) ->
-  external_intrinsics.callExternalOrIntrinsics TD M2' gse_fid 
-    (deckind_external eid_other) lp = Some (re, M2').
+  callExternalOrIntrinsics TD gl M2 gse_fid gse_typ Nil_list_typ
+    (deckind_external eid_other) lp = Some (re, events.E0, M2) ->
+  callExternalOrIntrinsics TD gl M2' gse_fid gse_typ Nil_list_typ
+    (deckind_external eid_other) lp = Some (re, events.E0, M2').
 
 Axiom store_doesnt_change_gmmd : forall M2 b2 ofs v0 Mem2' lc2 gl als
    bid0 eid0 bgv' egv' fs F B cs tmn S Ps EC TD v ck,
